compiler/backend/proofs/data_cseProofScript.sml
@@ -4,15 +4,6 @@ val _ = new_theory "data_cseProof";
 val _ = temp_bring_to_front_overload"get_vars"{Name="get_vars",Thy="dataSem"};
 val _ = temp_bring_to_front_overload"cut_env"{Name="cut_env",Thy="dataSem"};
 
-val state_rel_def = Define `
-state_rel (s1:'ffi dataSem$state) (t1:'ffi dataSem$state) (live:num_set) <=>
-          s1.code = t1.code /\ s1.clock = t1.clock /\ s1.space = t1.space /\
-s1.ffi = t1.ffi /\ s1.refs = t1.refs /\ s1.global = t1.global /\
-s1.handler = t1.handler /\ (LENGTH s1.stack = LENGTH t1.stack) /\
-(T)`;
-val cache_invariant = Define`
-cache_invariant (Cache entries) = T`
-
 val map_maybe_head = Q.prove(
 `!f x t. map_maybe f (x::t) =
 case f x of
@@ -98,7 +89,10 @@ rw[size_def, foldi_def] >-
 )
 );
 
-val size_foldi = save_thm("size_foldi_l1", size_foldi_l1 |> Q.SPEC `0` |> SIMP_RULE (srw_ss()) []);
+val size_foldi = save_thm("size_foldi_l1",
+                          size_foldi_l1
+                              |> Q.SPEC `0`
+                              |> SIMP_RULE (srw_ss()) []);
 
 val length_sum_map = Q.prove(
 `!l. LENGTH l = SUM (MAP (\_ . 1) l)`,
@@ -112,85 +106,249 @@ Induct_on `s` >> rw[foldi_def]
 
 val length_toAList_size_l = Q.prove(
 `!i s j l k.
-LENGTH (foldi (\k v a. (k,v)::a) j l s) + k = foldi (\k v a. 1 + a) i (LENGTH l + k) s`,
-rewrite_tac[length_sum_map, MAP] >>
-Induct_on `s` >-
-fs[LENGTH, toAList_def, foldi_def, length_sum_map] >-
-fs[LENGTH, toAList_def, foldi_def, length_sum_map] >-
-  (
-  rw[foldi_def] >>
-  last_x_assum (qspecl_then [`i + 2*sptree$lrnext i`, `j + 2 * sptree$lrnext j`, `l`] (ASSUME_TAC o GSYM) ) >> fs[]
-  ) >>
-rw[foldi_def] >>
-last_x_assum (qspecl_then [`i + 2*sptree$lrnext i`, `j + 2*sptree$lrnext j`, `l`, `k`] (ASSUME_TAC o GSYM)) >> fs[] >>
-rewrite_tac[ADD_ASSOC] >>
-once_rewrite_tac[ADD_COMM] >>
-rewrite_tac[ADD_ASSOC] >>
-rw[Once ADD_COMM] >>
-last_x_assum (qspecl_then [`sptree$lrnext i + i`, `j + sptree$lrnext j`, `(foldi (λk v a. (k,v)::a) (j + 2 * sptree$lrnext j) l s)`, `1 + k`] (ASSUME_TAC o GSYM) ) >> fs[] >>
-fs[] >>
-rw[MAP_foldi] >>
-rw[foldi_cons_k]
+  LENGTH (foldi (\k v a. (k,v)::a) j l s) + k = foldi (\k v a. 1 + a) i (LENGTH l + k) s`,
+  rewrite_tac[length_sum_map, MAP] >>
+  Induct_on `s` >> rw[foldi_def] >-
+    (last_x_assum (qspecl_then [`i + 2*sptree$lrnext i`, `j + 2 * sptree$lrnext j`, `l`] (ASSUME_TAC o GSYM) ) >> fs[]) >>
+  last_x_assum (qspecl_then [`i + 2*sptree$lrnext i`, `j + 2*sptree$lrnext j`, `l`, `k`] (ASSUME_TAC o GSYM)) >> fs[] >>
+  rewrite_tac[ADD_ASSOC] >>
+  once_rewrite_tac[ADD_COMM] >>
+  rewrite_tac[ADD_ASSOC] >>
+  rw[Once ADD_COMM] >>
+  last_x_assum (qspecl_then [`sptree$lrnext i + i`, `j + sptree$lrnext j`, `(foldi (λk v a. (k,v)::a) (j + 2 * sptree$lrnext j) l s)`, `1 + k`] (ASSUME_TAC o GSYM) ) >> fs[] >>
+  rw[MAP_foldi, foldi_cons_k]
 );
 
-val length_toAList_size_l1 = save_thm("tmp", length_toAList_size_l
+val length_toAList_size_l1 = length_toAList_size_l
         |> Q.SPECL [`i`, `s`, `j`, `[]`, `0`]
         |> SIMP_RULE list_ss []
-        |> GEN_ALL);
-
+        |> GEN_ALL;
 val length_toAList_size = Q.prove(
 `!s. LENGTH (toAList s) = size s`,
 rewrite_tac[size_foldi, toAList_def, length_toAList_size_l1, Once ADD_COMM]
 );
+val length_num_set_toList_size = Q.prove(
+`!s. LENGTH (num_set_toList s) = size s`,
+rw[num_set_toList_def, length_toAList_size]);
 
+val mul_div2 = Q.prove(
+`!a. (2 * a DIV 2 = a)`,
+Induct_on `a` >> rw [MULT_SUC, ADD_DIV_RWT]);
+val mul_suc_div2 = Q.prove(
+`!a. (2 * a + 1) DIV 2 = a`,
+Induct_on `a` >> rw [MULT_SUC, ADD_DIV_RWT, mul_div2]
+);
+val odd_double = Q.prove(
+`!x. ~(EVEN (2 * x + 1))`,
+Induct_on `x` >> rw[MULT_SUC, EVEN_ADD, EVEN_DOUBLE]);
 
-val cache_member_memoize = Q.prove(
-`!cache op args n.
-(cache_lookup op args cache = NONE)
-==>
-(cache_lookup op args (cache_memoize op args n cache) = SOME n)`,
-Cases_on `cache` >>
-Induct_on `l` >-
+val size_zero_lookup = Q.prove(
+`!s. (size s = 0) <=> (!x. lookup x s = NONE)`,
+Induct_on `s` >-
+fs[lookup_def] >-
+fs[lookup_def] >-
+(
+  Cases_on `size s = 0` >> Cases_on `size s' = 0` >> fs[] >> fs[] >-
   (
-  rw[cache_memoize_def] >>
-  rw[map_combine_def] >>
-  rw[map_alter_def] >>
-  rw[cache_memoize1_def] >>
-  rw[cache_lookup_def] >>
-  rw[num_set_head_may_def] >>
-  first_x_assum kall_tac >>
-  `MEM n (num_set_toList (insert n () LN))` by rw[member_num_set_toList_insert] >>
-  rw[num_set_toList_def]
-  CASE_TAC >> fs[num_set_toList_def] >>
-  `h = n \/ h <> n` by decide_tac >> simp[] >>
-
-  (* `MAP FST (toAList (insert n () LN)) = [n]` by *)
-  (* ( *)
-  (*   Induct_on `n` >- *)
-  (*   ( *)
-  (*     rw[Once insert_def] >> *)
-  (*     rw[toAList_def] >> *)
-  (*     rw[foldi_def] *)
-  (*   ) >> *)
-  (*   ( *)
-  (*     rw[Once insert_def] >> *)
-  (*     rw[toAList_def] >> *)
-  (*     rw[foldi_def] >> *)
-  (*     `n = 1` by ( *)
-  (*       ASSUME_TAC DIV_0_IMP_LT >> res_tac >> *)
-  (*       full_simp_tac std_ss [] >> *)
-  (*       `n = 0 \/ n = 1` by (decide_tac ) >- fs[EVEN] *)
-  (*     ) >> *)
-  (*     full_simp_tac std_ss [] >> *)
-  (*     rw[Once lrnext_def] *)
-  (*   ) *)
-  (* ) *)
-)
+    full_simp_tac std_ss [size_def, lookup_def] >>
+    rw[]
+  ) >-
+  (
+    rw[lookup_def] >>
+    EXISTS_TAC ``2 * x + 1: num`` >>
+    full_simp_tac arith_ss [odd_double, mul_div2] >>
+    Cases_on `lookup x s'` >> fs[]
+  ) >>
+  (
+    rw[lookup_def] >>
+    EXISTS_TAC ``2 * x + 2: num`` >>
+    full_simp_tac arith_ss [EVEN_ADD, EVEN_DOUBLE, mul_suc_div2] >>
+    Cases_on `lookup x s` >> fs[]
+  )
+) >>
+rw[size_def] >>
+exists_tac ``0:num`` >>
+rw[lookup_def]
 );
 
-val cache_lookup_none = Q.prove(
-
+val size_zero_domain = Q.prove(
+`!s. (size s = 0) <=> (!x. x ∉ domain s)`,
+rw[] >>
+Cases_on `size s = 0` >-
+(
+  CCONTR_TAC >>
+  fs[domain_lookup] >>
+  imp_res_tac size_zero_lookup >>
+  fs[]
+) >>
+rw[] >>
+Induct_on `s` >-
+fs[size_def] >-
+fs[size_def] >-
+(rw[] >> metis_tac []) >>
+rw[] >> metis_tac []
 );
+
+
+val num_set_toList_insert_singleton = Q.prove(
+`!s n. (size s = 0) ==> (num_set_toList (insert n () s) = [n])`,
+rw[] >>
+`MEM n (num_set_toList (insert n () s))` by rw[member_num_set_toList_insert] >>
+`size (insert n () s) = 1` by fs[size_insert, size_zero_domain] >>
+`LENGTH (num_set_toList (insert n () s)) = 1` by rw[size_insert, length_num_set_toList_size] >>
+Cases_on `num_set_toList (insert n () s)` >- fs[] >>
+Cases_on `t` >> fs[]
+);
+val num_set_toList_empty = Q.prove(
+`!s. (num_set_toList s = []) = (size s = 0)`,
+rw[GSYM length_num_set_toList_size]
+);
+
+val state_rel_def = Define `
+state_rel (s1:'ffi dataSem$state) (t1:'ffi dataSem$state) (cache:cache) <=>
+s1.code = t1.code /\ s1.clock = t1.clock /\
+s1.space = t1.space /\
+s1.ffi = t1.ffi /\
+s1.refs = t1.refs /\
+s1.global = t1.global /\
+s1.handler = t1.handler /\
+LENGTH s1.stack = LENGTH t1.stack /\
+(!x. lookup x s1.locals = lookup x t1.locals) /\
+(!op args. (cache_lookup op args cache = SOME v) ==> (
+
+
+      do_app op xs s1 = Rval (v, some_s)))
+`;
+
+val state_rel_ID = Q.prove(
+`!s live. state_rel s s live`,
+fs [state_rel_def]);
+
+(* copied and barely adapted from dataLive *)
+(* val evaluate_compile_A = Q.prove( *)
+(* `!c s1 res s2 l2 t1 l1 d. *)
+(* (evaluate (c, s1) = (res, s2)) /\ *)
+(* state_rel s1 t1 l1 /\ *)
+(* (compile_A c l2 = (d, l1)) /\ (res <> SOME (Rerr (Rabort Rtype_error))) /\ *)
+(* (!s3. (jump_exc s1 = SOME s3) ==> *)
+(*   ?t3. (jump_exc t1 = SOME t3) /\ state_rel s3 t3 empty_cache /\ *)
+(*   (t3.handler = s3.handler) /\ *)
+(*   (LENGTH t3.stack = LENGTH s3.stack)) ==> *)
+(*     ?t2. (evaluate (d, t1) = (res, t2)) /\ *)
+(*     state_rel s2 t2 (case res of NONE => l2 | _ => empty_cache)`, *)
+(* ); *)
+
+val pair_if = Q.prove(
+`((a,b) = if c then (a1, b1) else (a2, b2)) =
+((a = if c then a1 else a2) /\ (b = if c then b1 else b2))`,
+rw[]
+);
+
+val evaluate_compile_A = Q.prove(
+`!c s1 res s2 l2 t1 l1 d.
+(evaluate (c, s1) = (res, s2)) /\
+state_rel s1 t1 l1 /\
+(compile_A c l2 = (d, l1)) /\ (res <> SOME (Rerr (Rabort Rtype_error))) /\
+(!s3. (jump_exc s1 = SOME s3) ==>
+  ?t3. (jump_exc t1 = SOME t3) /\ state_rel s3 t3 empty_cache /\
+  (t3.handler = s3.handler) /\
+  (LENGTH t3.stack = LENGTH s3.stack)) ==>
+    ?t2. (evaluate (d, t1) = (res, t2)) /\
+    state_rel s2 t2 (case res of NONE => l2 | _ => empty_cache)`,
+once_rewrite_tac [EQ_SYM_EQ] >>
+recInduct evaluate_ind >>
+rpt STRIP_TAC >-
+    (* Skip *)
+  fs[compile_A_def, evaluate_def] >-
+    (* Move *)
+  (
+    fs[state_rel_def, compile_A_def, evaluate_def, get_var_def] >>
+    Cases_on `lookup src t1.locals` >>
+    fs [set_var_def, lookup_insert]
+  ) >-
+  (
+  (* Assign *)
+    fs[state_rel_def, compile_A_def, evaluate_def, get_var_def] >>
+    Cases_on `is_pure op` >-
+    (
+      fs[]
+        cheat
+      full_simp_tac list_ss []
+      rev_full_simp_tac list_ss []
+    )
+  )
+);
+
+(* val cache_member_memoize = Q.prove( *)
+(* `!cache op args n. *)
+(* (cache_lookup op args cache = NONE) *)
+(* ==> *)
+(* (cache_lookup op args (cache_memoize op args n cache) = SOME n)`, *)
+(*   Cases_on `cache` >> Induct_on `l` >- *)
+(*     rw[cache_memoize_def, map_combine_def, map_alter_def, cache_memoize1_def, cache_lookup_def, num_set_toList_insert_singleton, num_set_head_may_def] >> *)
+(*   fs[cache_memoize_def, map_combine_def] >> *)
+(*   Cases_on `h` >> *)
+(*   fs[map_alter_def, cache_memoize1_def] >> *)
+(*   rw[] >- *)
+(*     ( *)
+(*     rw[cache_lookup_def] >> *)
+(*     rw[cache_memoize2_def] >> *)
+(*     Cases_on `r` >- ( *)
+(*       rw[map_combine_def, Once map_alter_def] >> *)
+(*       rw[cache_memoize2_def] >> *)
+(*       rw[cache_lookup_def] >> *)
+(*       rw[num_set_head_may_def, num_set_toList_insert_singleton] *)
+(*     ) >> *)
+(*     Cases_on `h` >> *)
+(*     rw[map_combine_def, map_alter_def] >> *)
+(*     rw[cache_memoize2_def] >> *)
+(*     rw[cache_lookup_def] >> *)
+(*     rw[num_set_head_may_def] >> *)
+(*     `size r = 0` by *)
+(*     ( *)
+(*       fs[cache_lookup_def, num_set_head_may_def] >> *)
+(*       Cases_on `num_set_toList r` >> rw[num_set_toList_def, toAList_def, foldi_def] >> *)
+(*       `LENGTH (num_set_toList r) = 0` by fs [] >> *)
+(*       rw[length_num_set_toList_size] >> *)
+(*       ASSUME_TAC length_num_set_toList_size >> *)
+(*       asm_rewrite_tac[GSYM length_num_set_toList_size] >> *)
+(*       fs[] *)
+(*     ) >> *)
+(*     `size (insert n () r) = 1` by ( *)
+(*       fs[size_insert] >> *)
+(*       rw[] >> *)
+(*       imp_res_tac size_zero_domain >> fs[] *)
+(*       ) >> *)
+(*     imp_res_tac num_set_toList_insert_singleton >> *)
+(*     rw[] *)
+(*     ) >> *)
+(*     (* ntac 3 (first_x_assum kall_tac) >> *) *)
+(*     (* wrong! loop begins here! *) *)
+(*     Induct_on `t` >- *)
+(*       rw[map_combine_def, map_alter_def, cache_memoize2_def, num_set_head_may_def, num_set_toList_insert_singleton] >> *)
+(*     Cases_on `h` >> *)
+(*     rw[map_alter_def, cache_memoize2_def] >> *)
+(*     `size r' = 0` by ( *)
+(*       fs[cache_lookup_def, num_set_head_may_def] >> *)
+(*       rev_full_simp_tac std_ss [] >> *)
+(*       Cases_on `num_set_toList x` >- ( *)
+(*         fs[] *)
+(*         rw[length_num_set_toList_size] >> *)
+(*         ASSUME_TAC length_num_set_toList_size >> *)
+(*         asm_rewrite_tac[GSYM length_num_set_toList_size] >> *)
+(*         fs[] *)
+(*       ) >> *)
+(*       fs[] *)
+(*     ) >> *)
+(*     rw[num_set_head_may_def] *)
+(*     imp_res_tac num_set_toList_insert_singleton >> *)
+(*     fs[] *)
+(*     (* loop ends here *) *)
+(* ); *)
+
+(* val cache_lookup_none = Q.prove( *)
+
+(* ); *)
 
 
 val _ = export_theory();
